#+title: Assignment 6
#+HTML_MATHJAX: align: left indent: 2em
#+HTML_HEAD: <link rel="stylesheet" type="text/css" href="../../myStyle.css" />
#+OPTIONS: html-style:nil H:2 toc:2 todo:nil author:nil date:nil
#+HTML_LINK_HOME: ../../material.html
The following assignment is due *Thursday 3/27 by 8:00 PM*.  You'll
need to submit a ~pdf~ file on Gradescope.

* Soundness of IPL
Recall the proof system IPL:
#+begin_quote
\begin{align*}
\frac
{}
{\Gamma, \phi, \Delta \vdash \phi}
\text{(assumption)}
\qquad
\frac
{\Gamma \vdash \bot}
{\Gamma \vdash \phi}
\text{($\bot$-elim)}
\end{align*}
\begin{align*}
\frac
{\Gamma, \phi \vdash \psi}
{\Gamma \vdash \phi \to \psi}
\text{($\to$-intro)}
\qquad
\frac
{\Gamma \vdash \phi \to \psi \qquad \Gamma \vdash \phi}
{\Gamma \vdash \psi}
\text{($\to$-elim)}
\end{align*}

\begin{align*}
\frac
{\Gamma \vdash \phi \qquad \Gamma \vdash \psi}
{\Gamma \vdash \phi \land \psi}
\text{($\land$-intro)}
\qquad
\frac
{\Gamma \vdash \phi \land \psi}
{\Gamma \vdash \phi}
\text{($\land$-elim$_0$)}
\qquad
\frac
{\Gamma \vdash \phi \land \psi}
{\Gamma \vdash \phi}
\text{($\land$-elim$_1$)}
\end{align*}
\begin{align*}
\frac
{\Gamma \vdash \phi}
{\Gamma \vdash \phi \lor \psi}
\text{($\lor$-intro$_0$)}
\qquad
\frac
{\Gamma \vdash \psi}
{\Gamma \vdash \phi \lor \psi}
\text{($\lor$-intro$_1$)}
\end{align*}
\begin{align*}
\frac
{\Gamma \vdash \phi \lor \psi \qquad \Gamma, \phi \vdash \xi \qquad \Gamma, \psi \vdash \xi}
{\Gamma \vdash \xi}
\text{($\lor$-elim)}
\end{align*}
#+end_quote

Prove the soundness theorem for IPL. That is, prove that if $\Gamma
\vdash \phi$ according to the above rules, then $\Gamma \vDash \phi$.
You should use induction on the structure of the derivation of $\Gamma
\vdash \phi$.

* Weakening in STLC
Recall the type system STLC:

#+begin_quote
\begin{align*}
\frac
{}
{\Gamma, x : A, \Delta \vdash x : A}
\text{(assumption)}
\qquad
\frac
{\Gamma, x : A \vdash M : B}
{\Gamma \vdash \lambda x . M : A \to B}
\text{($\to$-intro)}
\end{align*}
\begin{align*}
\frac
{\Gamma \vdash M : A \to B \qquad \Gamma \vdash N : A}
{\Gamma \vdash M N : B}
\text{($\to$-elim)}
\end{align*}
#+end_quote

Prove that weakening is an admissible rule in STLC. Recall that the
weakening rule is written as:

\[
\frac
{\Gamma \vdash M : A}
{\Gamma, x : B \vdash M : A}
\text{(weakening)}
\]

where ùë• does not appear in Œì and ùêµ is a simple type.  You should prove
this by induction on the structure of the derivation of Œì ‚ä¢ ùëÄ ‚à∂ ùêµ.
(/Hint./ You may want to prove the stronger fact that we can introduce
a variable anywhere in the context Œì and not just at the end)

* A Variant of Linear Logic
Consider the following proof system:

#+begin_quote
\[
\frac
{}
{\phi \vdash \phi}
\text{(start)}
\qquad
\frac
{\Gamma \vdash \phi}
{\pi(\Gamma) \vdash \phi}
\text{(exchg)}
\]

\[
\frac
{\Gamma, \phi \vdash \psi}
{\Gamma \vdash \phi \to \psi}
\text{($\to$-intro)}
\qquad
\frac
{
\Gamma \vdash \phi \to \psi
\qquad
\Delta \vdash \phi
}
{
\Gamma, \Delta \vdash \psi
}
\text{($\to$-elim)}
\]
\[
\frac
{
\Gamma \vdash \phi
\qquad
\Delta \vdash \psi
}
{\Gamma, \Delta \vdash \phi \land \psi}
\text{($\land$-intro)}
\qquad
\frac
{
\Gamma \vdash \phi \land \psi
\qquad
\Delta, \phi, \psi \vdash \xi
}
{
\Gamma, \Delta \vdash \xi
}
\text{($\land$-elim)}
\]
\[
\frac
{\Gamma \vdash \phi}
{\Gamma \vdash \phi \land \phi}
\text{(clone)}
\qquad
\frac
{\Gamma \vdash \phi \land \psi}
{\Gamma \vdash \phi}
\text{(drop)}
\]
#+end_quote

Prove that this proof system is equivalent to the following proof
system (which may be thought of as a fragment of IPL over $\to$ and
$\land$):
#+begin_quote
\[
\frac
{}
{\phi \vdash \phi}
\text{(start)}
\qquad
\frac
{\Gamma \vdash \phi}
{\pi(\Gamma) \vdash \phi}
\text{(exchg)}
\qquad
\frac
{
\Gamma \vdash \phi
}
{
\Gamma, \psi \vdash \phi
}
\text{(weakn)}
\qquad
\frac
{\Gamma, \phi, \phi \vdash \psi}
{\Gamma, \phi \vdash \psi}
\text{(contr)}
\]

\begin{align*}
\frac
{\Gamma, \phi \vdash \psi}
{\Gamma \vdash \phi \to \psi}
\text{($\to$-intro)}
\qquad
\frac
{\Gamma \vdash \phi \to \psi \qquad \Delta \vdash \phi}
{\Gamma, \Delta \vdash \psi}
\text{($\to$-elim)}
\end{align*}

\begin{align*}
\frac
{\Gamma \vdash \phi \qquad \Delta \vdash \psi}
{\Gamma, \Delta \vdash \phi \land \psi}
\text{($\land$-intro)}
\qquad
\frac
{
\Gamma \vdash \phi \land \psi
\qquad
\Delta, \phi, \psi \vdash \xi
}
{
\Gamma, \Delta \vdash \xi
}
\text{($\land$-elim)}
\end{align*}
#+end_quote

This requires showing that the rules in one system are admissible in
the other.  This does not require structural induction.  You should be
able to build derivations which /simulate/ the rules given certain
assumptions (see the reading from this week for some examples of
this).  You may use without proof the following admissible rule in the
second system:

\[
\frac
{\Gamma \vdash \phi}
{\Delta \vdash \phi}
\text{(genContr)}
\]

where $\Delta$ is contained in $\Gamma$.

* Heap-Based Semantics

*(Optional)* Considing the following variant of a linear type
system. It is essentially the system which Curry-Howard corresponds to
the logic from the previous problem, but with an addition unit type so
that we can write non-trivial programs. Note that the ‚ä§-elimination
rule is trivial, but is required for the semantics so that we can
model allocation/deallocation.

#+begin_quote
syntax:
#+begin_src bnf
  <v>  ::= x | y | z | w | a | b | c | ...
  <t>  ::= ‚óè | <v> | Œª <v> . <t> | <t> <t> | <t> , <t>
	 | case <t> of <v> , <v> ‚Üí <t>
	 | case <t> of ‚óè ‚Üí <t>
	 | clone(<t>) | drop(<t>)
  <ty> ::= ‚ä§ | <ty> ‚àß <ty> | <ty> ‚Üí <ty>
#+end_src

type system:

\[
\frac
{}
{x : A \vdash x : A}
\text{(start)}
\qquad
\frac
{\Gamma \vdash M : A}
{\pi(\Gamma) \vdash M : A}
\text{(exchg)}
\]

\[
\frac
{}
{\vdash \bullet : \top}
\text{($\top$-intro)}
\qquad
\frac
{\Gamma \vdash M : \top
\qquad
\Delta \vdash N : A
}
{\Gamma, \Delta \vdash \texttt{case } M \texttt{ of } \bullet \to N : A}
\text{($\top$-elim)}
\]

\[
\frac
{\Gamma, x : A \vdash M : B}
{\Gamma \vdash \lambda x . M : A \to B}
\text{($\to$-intro)}
\qquad
\frac
{
\Gamma \vdash M : A \to B
\qquad
\Delta \vdash N : A
}
{
\Gamma, \Delta \vdash M N : B
}
\text{($\to$-elim)}
\]
\[
\hspace{-3mm}
\frac
{
\Gamma \vdash M : A
\qquad
\Delta \vdash N : B
}
{\Gamma, \Delta \vdash M, N : A \land B}
\text{($\land$-intro)}
\quad
\frac
{
\Gamma \vdash M: A \land B
\qquad
\Delta, x : A, y : B \vdash N : C
}
{
\Gamma, \Delta \vdash \texttt{case } M \texttt{ of } x, y \to N : C
}
\text{($\land$-elim)}
\]
\[
\frac
{\Gamma \vdash M : A}
{\Gamma \vdash \texttt{clone}(M) : A \land A}
\text{(clone)}
\qquad
\frac
{\Gamma \vdash M : A \land B}
{\Gamma \vdash \texttt{drop}(M): A}
\text{(drop)}
\]
#+end_quote

Following [[https://homepages.inf.ed.ac.uk/wadler/topics/linear-logic.html#linearop][this paper]] by Turner and Wadler, we can give a heap-based
semantics to this system.  The idea: we define a big-step relation $\{
H \} M \Downarrow \{ H \} x$ where $H$ is a unordered mapping from
variables to values (i.e., a unit, function, or pair of values).  This
mapping represents the heap, and the right-hand side of the relation
is always a variable, thought of as a pointer to a value on the heap.

I've taken some heavy liberties in defining this system, so we lose
many of the guarantees that the original paper proves, but it is
sufficient to model a simple version of ~clone~ and ~drop~.

In the following rules, /fresh/ means that there is no clash with
any variables that appear in the given expression.

#+begin_quote
values:
#+begin_src bnf
  <val> ::= Œª<v> . <e> | <val> , <val> | ‚óè
#+end_src

big-step semantics:

\[
\frac
{}
{\{H\} x \Downarrow \{ H \} x  }
\qquad
\frac
{\text{$y$ is fresh}}
{\{H\} \lambda x . M \Downarrow \{ H, y \mapsto \lambda x . M \} y}
\]
\[
\frac
{\text{$x$ is fresh}}
{\{H\} \bullet \Downarrow \{ H, x \mapsto \bullet\}x}
\qquad
\frac
{
\{H\} M \Downarrow \{ H', x \mapsto \bullet\} x
\qquad
\{H'\} N \Downarrow \{ H'' \}y
}
{
\{H\} \texttt{case } M \texttt{ of } \bullet \to N \Downarrow \{ H'' \}y
}
\qquad
\frac
{}
{}
\]
\[
\frac
{
\{H\} M \Downarrow \{ H' \} x
\qquad
\{H'\} N \Downarrow \{ H'', x \mapsto \lambda y. M' \}z
\qquad
\{H''\} M'[z / y] \Downarrow \{ H'''\} w
}
{
\{ H \} M N \Downarrow \{ H''' \} w
}
\]
\[
\frac
{
\{ H \} M \Downarrow \{ H' \} x
\qquad
\{ H' \} N \Downarrow \{ H'', x \mapsto v_1, y \mapsto v_2 \} y
}
{
\{ H \} (M, N) \Downarrow \{ H'', z \mapsto (v_1,  v_2) \} z
}
\]
\[
\hspace{-11mm}
\frac
{
\{ H \} M \Downarrow \{ H', z \mapsto (v_1, v_2) \} z
\qquad
\text{$q$, $r$ are fresh}
\qquad
\{ H', q \mapsto v_1, r \mapsto v_2 \} N[q / x] [r / y]  \Downarrow \{ H'' \} w
}
{
\{ H \} \texttt{case } M \texttt{ of } x, y \to N \Downarrow \{ H'' \}w
}
\]
\[
\frac
{
\{ H \} M \Downarrow \{ H', x \mapsto v \} x
}
{
\{ H \} \texttt{clone}(M) \Downarrow \{ H', x \mapsto (v, v) \} x
}
\]
\[
\frac
{
\{H\} M \Downarrow \{ H', x \mapsto (v_1, v_2) \} x
}
{
\{ H \} \texttt{drop}(M) \Downarrow \{ H', x \mapsto v_1 \} z
}
\]
#+end_quote

Give a derivation of the following judgment, also determining the heap $H$.

\[
\{\texttt{x} \mapsto \bullet \} \texttt{case clone(x) of x, y ‚Üí drop(x, y)} \Downarrow \{H\} \texttt{z}
\]

Note that, since variables are chosen to be fresh in many rules above,
it is not required that the derivation end in the variable ~z~
specifically, but it should be a variable which points to a value on
the heap.
